src/proof/k8s_io/api/apps/v1.v
@@ -1,0 +1,10 @@
+From New.proof.k8s_io.api.apps Require Export v1_init.
+
+From New.proof Require Import prelude empty_ffi pure_objects.
+
+Section proof.
+Context `{hG: !heapGS Σ} {go_ctx: GoContext}.
+
+
+
+End proof.
