src/proof/k8s_io/apimachinery/pkg/runtime/schema.v
@@ -1,0 +1,17 @@
+From New.proof.k8s_io.apimachinery.pkg.runtime Require Export schema_init.
+From New.proof Require Import prelude empty_ffi.
+
+Section proof.
+Context `{hG: !heapGS Σ} {go_ctx: GoContext}.
+
+Lemma wp_GroupVersion__WithKind (gv: schema.GroupVersion.t) kind:
+  {{{ is_pkg_init schema }}}
+    gv @ schema.GroupVersion.id @ "WithKind" #kind
+  {{{ gvk, RET #gvk;
+      ⌜ gvk.(schema.GroupVersionKind.Group') = gv.(schema.GroupVersion.Group') ∧
+        gvk.(schema.GroupVersionKind.Version') = gv.(schema.GroupVersion.Version') ∧
+        gvk.(schema.GroupVersionKind.Kind') = kind ⌝
+  }}}.
+Proof. wp_start. wp_auto. wp_end. Qed.
+
+End proof.
